Add executable FMP rejection fixtures

venom/defs/fmpWfPropsScript.sml
@@ -722,4 +722,347 @@ Proof
        fmp_positive_invoke_layout_wf, fmp_positive_context_wf]
 QED
 
+(* Closed negative fixtures: each changes one relevant root or seal condition. *)
+Definition fmp_bad_nonentry_initial_fn_def:
+  fmp_bad_nonentry_initial_fn =
+    mk_raw_function "bad_nonentry_initial"
+      [<| bb_label := "entry";
+          bb_instructions := [mk_inst 40 INITIAL_FMP [] ["x"]] |>]
+End
+
+Definition fmp_bad_nonentry_initial_ctx_def:
+  fmp_bad_nonentry_initial_ctx =
+    mk_venom_context [fmp_bad_nonentry_initial_fn] NONE
+End
+
+Definition fmp_bad_entry_param_sig_def:
+  fmp_bad_entry_param_sig =
+    <| fms_has_fmp_param := T; fms_publishes := F |>
+End
+
+Definition fmp_bad_entry_param_fn_def:
+  fmp_bad_entry_param_fn =
+    (mk_raw_function "bad_entry_param"
+      [<| bb_label := "entry";
+          bb_instructions := [mk_inst 41 FMP_PARAM [Lit 0w] ["x"]] |>])
+      with fn_fmp_signature := SOME fmp_bad_entry_param_sig
+End
+
+Definition fmp_bad_entry_param_ctx_def:
+  fmp_bad_entry_param_ctx =
+    mk_venom_context [fmp_bad_entry_param_fn] (SOME "bad_entry_param")
+End
+
+Theorem fmp_malformed_root_rejections_eval:
+  ~fmp_value_rooted fmp_bad_nonentry_initial_ctx fmp_positive_entry_sig
+     fmp_bad_nonentry_initial_fn "x" /\
+  ~fmp_value_rooted fmp_bad_entry_param_ctx fmp_bad_entry_param_sig
+     fmp_bad_entry_param_fn "x"
+Proof
+  EVAL_TAC >> simp[]
+QED
+
+Definition fmp_hidden_mismatch_sig_def:
+  fmp_hidden_mismatch_sig =
+    <| fms_has_fmp_param := F; fms_publishes := T |>
+End
+
+Definition fmp_hidden_mismatch_fn_def:
+  fmp_hidden_mismatch_fn =
+    fmp_positive_callee with
+      fn_fmp_signature := SOME fmp_hidden_mismatch_sig
+End
+
+Definition fmp_positive_callee_explicit_abi_def:
+  fmp_positive_callee_explicit_abi =
+    fmp_positive_callee with fn_call_abi :=
+      (fmp_positive_callee.fn_call_abi with
+         ica_user_return_count := SOME 1)
+End
+
+Definition fmp_publish_mismatch_sig_def:
+  fmp_publish_mismatch_sig =
+    <| fms_has_fmp_param := T; fms_publishes := F |>
+End
+
+Definition fmp_publish_mismatch_fn_def:
+  fmp_publish_mismatch_fn =
+    fmp_positive_callee_explicit_abi with
+      fn_fmp_signature := SOME fmp_publish_mismatch_sig
+End
+
+Definition fmp_absent_seal_fn_def:
+  fmp_absent_seal_fn =
+    fmp_positive_callee with fn_fmp_signature := NONE
+End
+
+Theorem fmp_malformed_seal_rejections_eval:
+  ~fmp_seal_layout_matches_fn fmp_hidden_mismatch_fn
+     fmp_hidden_mismatch_sig /\
+  fmp_seal_layout_matches_fn fmp_positive_callee_explicit_abi
+     fmp_positive_callee_sig /\
+  ~fmp_seal_layout_matches_fn fmp_publish_mismatch_fn
+     fmp_publish_mismatch_sig /\
+  ~call_abi_matches_fn fmp_absent_seal_fn
+Proof
+  EVAL_TAC
+QED
+
+
+Definition fmp_dangling_invoke_def:
+  fmp_dangling_invoke =
+    mk_inst 50 INVOKE
+      [Label "missing"; Lit 7w; Var "minus"] ["user_out"; "published"]
+End
+
+Definition fmp_short_input_invoke_def:
+  fmp_short_input_invoke =
+    mk_inst 51 INVOKE
+      [Label "callee"; Var "minus"] ["user_out"; "published"]
+End
+
+Definition fmp_short_output_invoke_def:
+  fmp_short_output_invoke =
+    mk_inst 52 INVOKE
+      [Label "callee"; Lit 7w; Var "minus"] ["user_out"]
+End
+
+Theorem fmp_positive_lookup_facts:
+  lookup_function "callee" fmp_positive_ctx.ctx_functions =
+    SOME fmp_positive_callee /\
+  lookup_function "missing" fmp_positive_ctx.ctx_functions = NONE
+Proof
+  EVAL_TAC
+QED
+
+Theorem fmp_malformed_invoke_arity_facts:
+  ~invoke_input_arity_ok fmp_positive_callee fmp_positive_callee_sig
+     fmp_short_input_invoke /\
+  ~fmp_invoke_output_arity_ok fmp_positive_callee fmp_positive_callee_sig
+     fmp_short_output_invoke
+Proof
+  EVAL_TAC
+QED
+
+Theorem fmp_malformed_invoke_layout_rejections_eval:
+  ~invoke_layout_wf fmp_positive_ctx fmp_dangling_invoke /\
+  ~invoke_layout_wf fmp_positive_ctx fmp_short_input_invoke /\
+  ~invoke_layout_wf fmp_positive_ctx fmp_short_output_invoke
+Proof
+  simp[invoke_layout_wf_def, fmp_dangling_invoke_def,
+       fmp_short_input_invoke_def, fmp_short_output_invoke_def,
+       venomInstTheory.mk_inst_def, fmp_positive_lookup_facts,
+       fmp_seal_layout_matches_fn_def, fmp_positive_signature_fields,
+       fmp_positive_callee_syntax_wf, fmp_malformed_invoke_arity_facts]
+  >> EVAL_TAC
+QED
+
+Definition fmp_unrooted_hidden_invoke_def:
+  fmp_unrooted_hidden_invoke =
+    mk_inst 53 INVOKE
+      [Label "callee"; Lit 7w; Var "ghost"] ["user_out"; "published"]
+End
+
+Definition fmp_unrooted_hidden_caller_def:
+  fmp_unrooted_hidden_caller =
+    (mk_raw_function "bad_hidden_caller"
+      [<| bb_label := "entry";
+          bb_instructions := [fmp_unrooted_hidden_invoke] |>]) with <|
+      fn_eom := SOME 0;
+      fn_fmp_signature := SOME fmp_positive_entry_sig
+    |>
+End
+
+Definition fmp_unrooted_hidden_ctx_def:
+  fmp_unrooted_hidden_ctx =
+    mk_venom_context
+      [fmp_unrooted_hidden_caller; fmp_positive_callee]
+      (SOME "bad_hidden_caller")
+End
+
+Theorem fmp_unrooted_hidden_lookup:
+  lookup_function "callee" fmp_unrooted_hidden_ctx.ctx_functions =
+    SOME fmp_positive_callee
+Proof
+  EVAL_TAC
+QED
+
+Theorem fmp_unrooted_hidden_layout_wf:
+  invoke_layout_wf fmp_unrooted_hidden_ctx fmp_unrooted_hidden_invoke
+Proof
+  simp[invoke_layout_wf_def, fmp_unrooted_hidden_invoke_def,
+       venomInstTheory.mk_inst_def]
+  >> qexistsl [`fmp_positive_callee`, `fmp_positive_callee_sig`]
+  >> conj_tac >- simp[fmp_unrooted_hidden_lookup]
+  >> conj_tac >-
+    simp[fmp_seal_layout_matches_fn_def,
+         cj 2 fmp_positive_signature_fields,
+         fmp_positive_callee_syntax_wf]
+  >> conj_tac >- EVAL_TAC
+  >> EVAL_TAC
+QED
+
+Theorem fmp_unrooted_hidden_value_rejected:
+  ~fmp_value_rooted fmp_unrooted_hidden_ctx fmp_positive_entry_sig
+     fmp_unrooted_hidden_caller "ghost"
+Proof
+  EVAL_TAC >> simp[]
+QED
+
+Theorem fmp_unrooted_hidden_invoke_facts:
+  fmp_unrooted_hidden_invoke.inst_opcode = INVOKE /\
+  fmp_unrooted_hidden_invoke.inst_operands =
+    [Label "callee"; Lit 7w; Var "ghost"] /\
+  invoke_input_arity_ok fmp_positive_callee fmp_positive_callee_sig
+    fmp_unrooted_hidden_invoke /\
+  fmp_invoke_output_arity_ok fmp_positive_callee fmp_positive_callee_sig
+    fmp_unrooted_hidden_invoke /\
+  fmp_positive_callee_sig.fms_has_fmp_param /\
+  EL (LENGTH (fn_user_param_insts fmp_positive_callee))
+    [Lit 7w; Var "ghost"] = Var "ghost"
+Proof
+  EVAL_TAC
+QED
+
+Theorem fmp_unrooted_hidden_rejection_eval:
+  invoke_layout_wf fmp_unrooted_hidden_ctx fmp_unrooted_hidden_invoke /\
+  ~fmp_runner_inst_wf fmp_unrooted_hidden_ctx fmp_positive_entry_sig
+     fmp_unrooted_hidden_caller fmp_unrooted_hidden_invoke
+Proof
+  simp[fmp_unrooted_hidden_layout_wf, fmp_runner_inst_wf_def,
+       fmp_bump_consumer_wf_def, fmp_invoke_consumer_wf_def,
+       fmp_return_consumer_wf_def, fmp_unrooted_hidden_invoke_facts,
+       fmp_unrooted_hidden_lookup, fmp_seal_layout_matches_fn_def,
+       cj 2 fmp_positive_signature_fields,
+       fmp_positive_callee_syntax_wf, fmp_unrooted_hidden_value_rejected]
+QED
+Definition fmp_unrooted_adopted_fn_def:
+  fmp_unrooted_adopted_fn =
+    (mk_raw_function "bad_adopted"
+      [<| bb_label := "entry";
+          bb_instructions :=
+            [mk_inst 60 PARAM [Lit 0w] ["cu"];
+             mk_inst 61 FMP_PARAM [Lit 1w] ["cfmp"];
+             mk_inst 62 RETPC_PARAM [Lit 2w] ["crpc"];
+             mk_inst 63 ADD [Var "cfmp"; Lit 1w] ["cadopt"];
+             mk_inst 64 RET [Var "cu"; Var "ghost"; Var "crpc"] []] |>])
+      with <| fn_eom := SOME 0;
+              fn_fmp_signature := SOME fmp_positive_callee_sig |>
+End
+
+Definition fmp_unrooted_adopted_ctx_def:
+  fmp_unrooted_adopted_ctx =
+    mk_venom_context [fmp_unrooted_adopted_fn] NONE
+End
+
+Definition fmp_unrooted_adopted_ret_def:
+  fmp_unrooted_adopted_ret =
+    mk_inst 64 RET [Var "cu"; Var "ghost"; Var "crpc"] []
+End
+
+Theorem fmp_unrooted_adopted_rejection_eval:
+  fmp_signature_syntax_wf fmp_positive_callee_sig
+    fmp_unrooted_adopted_fn /\
+  ~fmp_runner_inst_wf fmp_unrooted_adopted_ctx
+     fmp_positive_callee_sig fmp_unrooted_adopted_fn
+     fmp_unrooted_adopted_ret
+Proof
+  EVAL_TAC >> simp[venomInstTheory.operand_var_def]
+QED
+
+Definition fmp_misordered_return_fn_def:
+  fmp_misordered_return_fn =
+    (mk_raw_function "bad_return_order"
+      [<| bb_label := "entry";
+          bb_instructions :=
+            [mk_inst 65 PARAM [Lit 0w] ["cu"];
+             mk_inst 66 FMP_PARAM [Lit 1w] ["cfmp"];
+             mk_inst 67 RETPC_PARAM [Lit 2w] ["crpc"];
+             mk_inst 68 ADD [Var "cfmp"; Lit 1w] ["cadopt"];
+             mk_inst 69 RET [Var "cu"; Var "crpc"; Var "cadopt"] []] |>])
+      with <| fn_eom := SOME 0;
+              fn_fmp_signature := SOME fmp_positive_callee_sig |>
+End
+
+Definition fmp_misordered_return_ctx_def:
+  fmp_misordered_return_ctx =
+    mk_venom_context [fmp_misordered_return_fn] NONE
+End
+
+Definition fmp_misordered_return_inst_def:
+  fmp_misordered_return_inst =
+    mk_inst 69 RET [Var "cu"; Var "crpc"; Var "cadopt"] []
+End
+
+Definition fmp_bad_abi_return_fn_def:
+  fmp_bad_abi_return_fn =
+    fmp_positive_callee with fn_call_abi :=
+      (fmp_positive_callee.fn_call_abi with
+         ica_user_return_count := SOME 2)
+End
+
+Theorem fmp_malformed_return_layout_rejections_eval:
+  ~lowered_return_inst_layout_wf T 1
+     (mk_inst 70 RET [Var "u"; Var "rpc"] []) /\
+  ~lowered_return_inst_layout_wf T 1
+     (mk_inst 71 RET [Var "u"; Var "a"; Var "x"; Var "rpc"] []) /\
+  ~lowered_return_inst_layout_wf F 1
+     (mk_inst 72 RET [Var "rpc"] []) /\
+  lowered_return_inst_layout_wf T 1 fmp_misordered_return_inst /\
+  ~fmp_runner_inst_wf fmp_misordered_return_ctx
+     fmp_positive_callee_sig fmp_misordered_return_fn
+     fmp_misordered_return_inst /\
+  ~fmp_return_abi_matches fmp_positive_callee_sig fmp_bad_abi_return_fn
+Proof
+  EVAL_TAC >> simp[venomInstTheory.operand_var_def]
+QED
+
+Definition fmp_missing_eom_fn_def:
+  fmp_missing_eom_fn =
+    fmp_positive_entry with fn_eom := NONE
+End
+
+Definition fmp_missing_eom_ctx_def:
+  fmp_missing_eom_ctx =
+    mk_venom_context [fmp_missing_eom_fn] (SOME "entry")
+End
+
+Definition fmp_unconcretized_static_fn_def:
+  fmp_unconcretized_static_fn =
+    (mk_raw_function "bad_static"
+      [<| bb_label := "entry";
+          bb_instructions := [mk_inst 80 ALLOCA [Lit 32w] ["slot"]] |>])
+      with <| fn_eom := SOME 0;
+              fn_fmp_signature := SOME fmp_positive_entry_sig |>
+End
+
+Definition fmp_unconcretized_static_ctx_def:
+  fmp_unconcretized_static_ctx =
+    mk_venom_context [fmp_unconcretized_static_fn] (SOME "bad_static")
+End
+
+Theorem fmp_missing_eom_static_rejection:
+  ~concretized_static_layouts_wf fmp_missing_eom_ctx
+Proof
+  simp[staticLayoutWfTheory.concretized_static_layouts_wf_def,
+       fmp_missing_eom_ctx_def,
+       venomInstTheory.mk_venom_context_def, fmp_missing_eom_fn_def]
+QED
+
+Theorem fmp_unconcretized_static_layout_rejection:
+  ~concretized_static_layouts_wf fmp_unconcretized_static_ctx
+Proof
+  EVAL_TAC >> simp[venomInstTheory.fn_insts_blocks_def]
+QED
+
+Theorem fmp_eom_and_static_rejections_eval:
+  ~concretized_static_layouts_wf fmp_missing_eom_ctx /\
+  ~fmp_lowered_context_wf fmp_missing_eom_ctx /\
+  ~concretized_static_layouts_wf fmp_unconcretized_static_ctx /\
+  ~fmp_lowered_context_wf fmp_unconcretized_static_ctx
+Proof
+  simp[fmp_missing_eom_static_rejection,
+       fmp_unconcretized_static_layout_rejection,
+       fmp_lowered_context_wf_def]
+QED
 val _ = export_theory();
